isabelle/RulesNonTrivial.thy
@@ -1,0 +1,218 @@
+theory RulesNonTrivial
+imports Rules  SubstContext
+begin
+
+section \<open>A relation is non-trivial if x \<rightarrow> x does not hold\<close>
+
+definition rel_non_trivial :: "red \<Rightarrow> bool"  where
+  "rel_non_trivial R \<longleftrightarrow> (\<forall> x. \<not> R x x)"
+
+lemma rel_non_trivial_sup2:
+  assumes "rel_non_trivial R" and "rel_non_trivial S"
+  shows "rel_non_trivial (R \<squnion> S)"
+  using assms by (auto simp add: rel_non_trivial_def)
+
+section \<open>The closure context preserves non-trivialness\<close>
+
+lemma rel_non_trivial_cc:
+  assumes "rel_non_trivial R"
+  shows "rel_non_trivial (cc R)"
+  using assms 
+by (auto simp add: rel_non_trivial_def elim!: cc.cases)
+
+section \<open>The Verse rules are non-trivial\<close>
+
+lemma rel_non_trivial_rule_PAdd: "rel_non_trivial rule_PAdd"
+  by (auto simp add: rel_non_trivial_def elim!: rule_PAdd.cases)
+
+lemma rel_non_trivial_rule_PGt: "rel_non_trivial rule_PGt"
+  by (auto simp add: rel_non_trivial_def elim!: rule_PGt.cases)
+
+lemma rel_non_trivial_rule_App_Beta: "rel_non_trivial rule_App_Beta"
+  by (auto simp add: rel_non_trivial_def elim!: rule_App_Beta.cases simp add: occursV_liftV)
+
+lemma rel_non_trivial_rule_App_Tup: "rel_non_trivial rule_App_Tup" 
+  apply (auto simp add: rel_non_trivial_def elim!: rule_App_Tup.cases)
+  apply (case_tac vs; simp)
+  apply (case_tac list; simp)
+  done
+
+lemma rel_non_trivial_rule_ULit: "rel_non_trivial rule_ULit"
+  by (auto simp add: rel_non_trivial_def elim!: rule_ULit.cases)
+
+lemma rel_non_trivial_rule_UTup: "rel_non_trivial rule_UTup"
+  apply (auto simp add: rel_non_trivial_def elim!: rule_UTup.cases in_set_zipE)
+  apply (case_tac vs1; simp)
+  apply (case_tac vs2; simp)
+  apply (case_tac list; simp)
+  apply (case_tac lista; simp)
+  done
+
+lemma rel_non_trivial_rule_UX: "rel_non_trivial rule_UX"
+  by (auto simp add: rel_non_trivial_def elim!: rule_UX.cases)
+
+lemma rel_non_trivial_rule_UXOccurs: "rel_non_trivial rule_UXOccurs"
+  by (auto simp add: rel_non_trivial_def elim!: rule_UXOccurs.cases)
+
+lemma map_eq:
+  "xs = map f xs \<longleftrightarrow> (\<forall> x \<in> set xs. x = f x)"
+  by (induction xs) auto
+
+lemma appVCE_substVCE_eq[simp]:
+  "appVCE vce e1 = appVCE (substVCE n v vce) e2 \<longleftrightarrow> vce = substVCE n v vce \<and> e1 = e2"
+by (cases vce) auto
+
+lemma appVC'_substVC_eq[simp]:
+  "appVC' vc e1 = appVC' (substVC n v vc) e2 \<longleftrightarrow> vc = substVC n v vc \<and> e1 = e2"
+by (induction vc arbitrary: n v e1 e2) (auto simp add: substVC_def appVC'_def)
+
+lemma appVC_substVC_eq[simp]:
+  "appVC vc e1 = appVC (substVC n v vc) e2 \<longleftrightarrow> vc = substVC n v vc \<and> e1 = e2"
+by (simp add:  appVC_def)
+
+lemma appECE_substECE_eq[simp]:
+  "appECE ece e1 = appECE (substECE n v ece) e2 \<longleftrightarrow> ece = substECE n v ece \<and> e1 = e2"
+by (cases ece) auto
+
+lemma appEC_substEC_eq[simp]:
+  "appEC ec e1 = appEC (substEC n v ec) e2 \<longleftrightarrow> ec = substEC n v ec \<and> e1 = e2"
+  by (induction n v ec arbitrary: e1 e2 rule: substEC.induct)
+     (auto simp add: appEC_def)
+
+lemma substE_eq[simp]:
+  "e = substE n v e \<longleftrightarrow> (occursE n e \<longrightarrow> v = Var n)" 
+and  substV_eq[simp]:
+  "v' = substV n v v' \<longleftrightarrow> (occursV n v' \<longrightarrow> v = Var n)"
+by(induction n v e and n v v' rule: substE_substV.induct) (auto simp add: map_eq)
+
+lemma substVCE_eq[simp]:
+  "vce = substVCE n v vce \<longleftrightarrow> (occursVCE n vce \<longrightarrow> v = Var n)"
+by (induction vce) (auto simp add: map_eq)
+
+lemma substVC_eq[simp]:
+  "vc = substVC n v vc \<longleftrightarrow> (occursVC n vc \<longrightarrow> v = Var n)"
+by (auto simp add: substVC_def occursVC_def map_eq)
+
+lemma substECE_eq[simp]:
+  "ece = substECE n v ece \<longleftrightarrow> (occursECE n ece \<longrightarrow> v = Var n)"
+by (cases ece) (auto simp add: occursECE_def)
+
+lemma substEC_eq[simp]:
+  "ec = substEC n v ec \<longleftrightarrow> (occursEC n ec \<longrightarrow> v = Var n)"
+by (induction n v ec rule: substEC.induct) (auto simp add: )
+
+lemma rel_non_trivial_rule_Subst: "rel_non_trivial rule_Subst"
+  by (auto simp add: rel_non_trivial_def elim!: rule_Subst.cases)
+
+lemma size_exp_substE_Var[simp]: "size_exp (substE n (Var k) e) = size_exp e"
+  sorry
+
+lemma size_exp_liftE[simp]: "size_exp (liftE n k e) = size_exp e"
+  sorry
+
+
+lemma rel_non_trivial_rule_SubstRec: "rel_non_trivial rule_SubstRec"
+  apply (auto simp add: rel_non_trivial_def elim!: rule_SubstRec.cases)
+  apply (drule arg_cong[where f =  size_exp])
+  apply (auto)
+  done
+
+lemma occursEC_replicate_CDef[simp]: "\<not> occursEC k (replicate n CDef)"
+  by (induction n arbitrary: k) (auto simp add: occursECE_def)
+
+lemma rel_non_trivial_rule_DefEliml: "rel_non_trivial rule_DefEliml"
+  by (auto simp add: rel_non_trivial_def elim!: rule_DefEliml.cases
+        simp add: occursE_liftE)
+
+lemma rel_non_trivial_rule_DefElimr: "rel_non_trivial rule_DefElimr"
+  by (auto simp add: rel_non_trivial_def elim!: rule_DefElimr.cases
+        simp add: occursE_liftE)
+
+lemma rel_non_trivial_rule_Swap: "rel_non_trivial rule_Swap"
+  by (auto simp add: rel_non_trivial_def elim!: rule_Swap.cases)
+
+lemma rel_non_trivial_rule_DefFloat: "rel_non_trivial rule_DefFloat"
+  by (auto simp add: rel_non_trivial_def elim!: rule_DefFloat.cases)
+
+lemma rel_non_trivial_rule_Seq: "rel_non_trivial rule_Seq"
+  by (auto simp add: rel_non_trivial_def elim!: rule_Seq.cases)
+
+lemma rel_non_trivial_rule_Unify_Seql: "rel_non_trivial rule_Unify_Seql"
+  by (auto simp add: rel_non_trivial_def elim!: rule_Unify_Seql.cases)
+
+lemma rel_non_trivial_rule_Unify_Seqr: "rel_non_trivial rule_Unify_Seqr"
+  by (auto simp add: rel_non_trivial_def elim!: rule_Unify_Seqr.cases)
+
+lemma rel_non_trivial_rule_Unify_Unifyl: "rel_non_trivial rule_Unify_Unifyl"
+  by (auto simp add: rel_non_trivial_def elim!: rule_Unify_Unifyl.cases simp add: occursE_liftE)
+
+lemma rel_non_trivial_rule_Unify_Unifyr: "rel_non_trivial rule_Unify_Unifyr"
+  by (auto simp add: rel_non_trivial_def elim!: rule_Unify_Unifyr.cases simp add: occursE_liftE)
+
+lemma rel_non_trivial_rule_DefFail: "rel_non_trivial rule_DefFail"
+  by (auto simp add: rel_non_trivial_def elim!: rule_DefFail.cases)
+
+lemma rel_non_trivial_rule_Fail: "rel_non_trivial rule_Fail"
+  by (auto simp add: rel_non_trivial_def elim!: rule_Fail.cases)
+
+lemma rel_non_trivial_rule_OneFail: "rel_non_trivial rule_OneFail"
+  by (auto simp add: rel_non_trivial_def elim!: rule_OneFail.cases)
+
+lemma rel_non_trivial_rule_OneChoice: "rel_non_trivial rule_OneChoice"
+  by (auto simp add: rel_non_trivial_def elim!: rule_OneChoice.cases)
+
+lemma rel_non_trivial_rule_OneValue: "rel_non_trivial rule_OneValue"
+  by (auto simp add: rel_non_trivial_def elim!: rule_OneValue.cases)
+
+lemma rel_non_trivial_rule_All: "rel_non_trivial rule_All"
+  by (auto simp add: rel_non_trivial_def elim!: rule_All.cases)
+
+lemma rel_non_trivial_rule_FailL: "rel_non_trivial rule_FailL"
+  by (auto simp add: rel_non_trivial_def elim!: rule_FailL.cases)
+
+lemma rel_non_trivial_rule_FailR: "rel_non_trivial rule_FailR"
+  by (auto simp add: rel_non_trivial_def elim!: rule_FailR.cases)
+
+lemma rel_non_trivial_rule_AssocChoice: "rel_non_trivial rule_AssocChoice"
+  by (auto simp add: rel_non_trivial_def elim!: rule_AssocChoice.cases)
+
+lemma rel_non_trivial_rule_Choose: "rel_non_trivial rule_Choose"
+  by (auto simp add: rel_non_trivial_def elim!: rule_Choose.cases)
+
+theorem ARs_non_trivial: "rel_non_trivial ARs"
+unfolding ARs_def
+by (intro rel_non_trivial_sup2
+   rel_non_trivial_rule_PAdd
+   rel_non_trivial_rule_PGt
+   rel_non_trivial_rule_App_Beta
+   rel_non_trivial_rule_App_Tup
+   rel_non_trivial_rule_ULit
+   rel_non_trivial_rule_UTup
+   rel_non_trivial_rule_UX
+   rel_non_trivial_rule_UXOccurs
+   rel_non_trivial_rule_Subst
+   rel_non_trivial_rule_SubstRec
+   rel_non_trivial_rule_DefEliml
+   rel_non_trivial_rule_DefElimr
+   rel_non_trivial_rule_Swap
+   rel_non_trivial_rule_DefFloat
+   rel_non_trivial_rule_Seq
+   rel_non_trivial_rule_Unify_Seql
+   rel_non_trivial_rule_Unify_Seqr
+   rel_non_trivial_rule_Unify_Unifyl
+   rel_non_trivial_rule_Unify_Unifyr
+   rel_non_trivial_rule_DefFail
+   rel_non_trivial_rule_Fail
+   rel_non_trivial_rule_OneFail
+   rel_non_trivial_rule_OneChoice
+   rel_non_trivial_rule_OneValue
+   rel_non_trivial_rule_All
+   rel_non_trivial_rule_FailL
+   rel_non_trivial_rule_FailR
+   rel_non_trivial_rule_AssocChoice
+   rel_non_trivial_rule_Choose
+)
+
+
+
+end
